src/Init/Prelude.lean
@@ -2568,7 +2568,9 @@ structure Array (α : Type u) where
   /--
   Converts a `List α` into an `Array α`.
 
-  At runtime, this constructor is implemented by `List.toArray` and is O(n) in the length of the
+  You can also use the synonym `List.toArray` when dot notation is convenient.
+
+  At runtime, this constructor is implemented by `List.toArrayImpl` and is O(n) in the length of the
   list.
   -/
   mk ::
@@ -2727,8 +2729,8 @@ def List.redLength : List α → Nat
 /-- Convert a `List α` into an `Array α`. This is O(n) in the length of the list.  -/
 -- This function is exported to C, where it is called by `Array.mk`
 -- (the constructor) to implement this functionality.
-@[inline, match_pattern, pp_nodot, export lean_list_to_array]
-def List.toArray (as : List α) : Array α :=
+@[inline, match_pattern, pp_nodot, export lean_list_to_array_impl]
+private def List.toArrayImpl (as : List α) : Array α :=
   as.toArrayAux (Array.mkEmpty as.redLength)
 
 /-- The typeclass which supplies the `>>=` "bind" function. See `Monad`. -/
